Modified palindrome proof kind of coming along?

theories/palindrome/palindrome_modified.v
@@ -14,12 +14,12 @@ Open Scope volpic_notation.
 Import ListNotations.
 
 Definition string_subscript (s : string) (idx : Z) : Z :=
-	match String.get (Z.to_nat idx) s with 
+	match String.get (Z.to_nat idx - 1) s with 
 	| None => -1
 	| Some a => Z.of_nat (Ascii.nat_of_ascii a)
 	end.
 
-Definition ispalindrome (VP_store: store) := 
+Definition ispalindrome (VP_store: store) loop_limit := 
 	let VP_poison := false in
 	let (VP_store,VP_poison) := 
 		(if (negb VP_poison) then
@@ -31,32 +31,383 @@ Definition ispalindrome (VP_store: store) :=
  			 (update VP_store "VP_LEN" (VInteger (Z.of_nat (String.length (get_string VP_store "VP_STR")))),VP_poison) 
 		else
  			(VP_store,true)) in
-	let (VP_store,VP_poison) := 
 		(if (negb VP_poison) then
  			 (match 
-(let going_up := 1 <? get_int VP_store "VP_LEN" / 2 in
-		let bounds_op := (if going_up then Z.leb else Z.geb) in
-		let iter_op := (if going_up then (Z.add 1) else (Z.sub 1)) in
+		(let going_up := 1 <? get_int VP_store "VP_LEN" / 2 in
+		let bounds_op := Z.leb in
+		let iter_op := Z.add 1 in
 		let VP_store := update VP_store "VP_I" (VInteger ( 1 )) in
-while ( fun VP_store => bounds_op (get_int VP_store "VP_I") (get_int VP_store "VP_LEN" / 2) ) with VP_store upto 1000%nat begin fun VP_store => 			
-let VP_store := if (string_subscript (get_string VP_store "VP_STR") (get_int VP_store "VP_I") !=? string_subscript (get_string VP_store "VP_STR") (get_int VP_store "VP_LEN" - get_int VP_store "VP_I" + 1)) then
- 	 ((*Block: next 2 statements*)
-			let VP_store := update VP_store "VP_result" (VInteger ( 0 )) in
-			let VP_broken := true in VP_store) 
-else
- 	((*nothing and mid-seq*) VP_store) in
-		let VP_store := update VP_store "VP_I" (VInteger (iter_op (get_int VP_store "VP_I"))) in VP_store end) with 
+			while ( fun VP_store => bounds_op (get_int VP_store "VP_I") (get_int VP_store "VP_LEN" / 2) ) with VP_store upto loop_limit 
+			begin fun VP_store => 
+			(* VP_result = 1 /\ VP_I <= VP_LEN / 2*)
+			let VP_store := if (string_subscript (get_string VP_store "VP_STR") (get_int VP_store "VP_I") !=? string_subscript (get_string VP_store "VP_STR") (get_int VP_store "VP_LEN" - get_int VP_store "VP_I" + 1)) then
+				((*Block: next 2 statements*)
+						let VP_store := update VP_store "VP_result" (VInteger ( 0 ))in
+						let VP_broken := true in VP_store) 
+			else
+				((*nothing and mid-seq*) VP_store) in
+					let VP_store := update VP_store "VP_I" (VInteger (iter_op (get_int VP_store "VP_I"))) in VP_store 
+			end) 
+		(* VP_result = 1 /\ ~ (VP_I <= VP_LEN / 2) *)
+		with
  		 | None => (VP_store,true)
-		 | Some VP_store' => (VP_store',VP_poison)
+		 | Some VP_store => (VP_store,VP_poison)
 		 	 end) 
 		else
- 			(VP_store,true)) in
-VP_store.
+ 			(VP_store,true)).
 
-Compute ispalindrome (update fresh_store "VP_STR" (VString "aa")) "VP_result".
+Compute fst (ispalindrome (update fresh_store "VP_STR" (VString "aaa")) 1) "VP_result".
 
 Extraction "palindrome.ml" ispalindrome.
 
-(*Failed to convert $main: Couldn't find key "value" in data list*)
+Require Import Ascii.
 
-Compute (main fresh_store).
+Inductive pal : string -> Prop :=
+| pal_nil : pal EmptyString
+| pal_single : forall (x : ascii), pal (String x EmptyString)
+| pal_ht : forall (h : ascii) (t : string), 
+	pal t -> pal ((String h t) ++ (String h EmptyString)).
+
+Definition reverse (s : string) :=
+	string_of_list_ascii (rev (list_ascii_of_string s)).
+
+Lemma string_of_list_ascii_distr : forall l1 l2,
+	string_of_list_ascii (l1 ++ l2) = 
+		string_of_list_ascii l1 ++ string_of_list_ascii l2.
+Proof.
+	induction l1; intros; auto.
+	simpl in *. now rewrite IHl1.
+Qed.
+
+Lemma rev_String : forall a s,
+	reverse (String a s) = reverse s ++ (String a EmptyString).
+Proof.
+	intros. generalize dependent a.
+	induction s; simpl in *; intros.
+	reflexivity.
+	rewrite IHs; simpl in *. unfold reverse; simpl.
+	now repeat rewrite string_of_list_ascii_distr; simpl.
+Qed.
+
+Lemma String_app_assoc : forall a s1 s2,
+	String a (s1 ++ s2) = (String a s1) ++ s2.
+Proof.
+	intros. destruct s1; reflexivity.
+Qed.
+
+Lemma app_assoc : forall s1 s2 s3,
+	s1 ++ (s2 ++ s3) = (s1 ++ s2) ++ s3.
+Proof.
+	induction s1; intros; simpl in *.
+	reflexivity.
+	now rewrite IHs1.
+Qed.
+
+Theorem pal_app_rev : forall (s : string),
+  pal (s ++ (reverse s)).
+Proof.
+    induction s; simpl.
+    constructor.
+	rewrite rev_String. replace (String a (s ++ reverse s ++ String a "")) with 
+		(String a (s ++ reverse s) ++ String a ""). now constructor.
+	now rewrite String_app_assoc, <- app_assoc, <- String_app_assoc.
+Qed.
+
+Lemma app_empty_r : forall s,
+	s ++ "" = s.
+Proof.
+	induction s; simpl.
+	reflexivity. now rewrite IHs.
+Qed.
+
+Lemma reverse_app_distr : forall s1 s2,
+	reverse (s1 ++ s2) = reverse s2 ++ reverse s1.
+Proof.
+	induction s1; intros; simpl in *. 
+	unfold reverse at 3. simpl. now rewrite app_empty_r.
+	rewrite String_app_assoc, rev_String, app_assoc, <- IHs1.
+	unfold reverse; simpl. now rewrite string_of_list_ascii_distr.
+Qed.
+
+Theorem pal_rev : forall (s: string), 
+    pal s -> s = reverse s.
+Proof.
+    intros. induction H; simpl in *; try reflexivity.
+    now rewrite rev_String, reverse_app_distr, <- IHpal.
+Qed.
+
+Lemma palindrome_cons : forall x s,
+    pal s -> pal ((String x s) ++ (String x "")).
+Proof.
+    induction s; intros.
+    - apply pal_app_rev.
+    - now apply pal_ht.
+Qed.
+
+Lemma split_last : forall s, 
+    s = "" \/ exists x p, s = p ++ (String x "").
+Proof.
+    induction s.
+    - now left.
+    - right. destruct IHs; subst.
+        -- now exists a, "".
+        -- destruct H, H; subst. now exists x, (String a x0).
+Qed.
+
+Require Import Nat.
+
+Lemma length_app_distr : forall s1 s2,
+	String.length (s1 ++ s2) = (String.length s1 + String.length s2)%nat.
+Proof.
+	induction s1; intros; simpl in *.
+	reflexivity.
+	now rewrite IHs1.
+Qed.
+
+Theorem plus_le : forall n1 n2 m,
+    (n1 + n2 <= m)%nat ->
+    (n1 <= m)%nat /\ (n2 <= m)%nat.
+Proof.
+    induction n1; intros; split.
+    apply Nat.le_0_l. assumption.
+    apply (Nat.le_trans _ (S n1 + n2) _).
+    apply Nat.le_add_r. assumption.
+    apply (Nat.le_trans _ (S n1 + n2) _).
+    rewrite Nat.add_comm. apply Nat.le_add_r. assumption.
+Qed.
+
+Lemma length_app_le :
+    forall s1 s2 n,
+    (String.length (s1 ++ s2) <= n)%nat ->
+    (String.length s1 <= n)%nat /\ (String.length s2 <= n)%nat.
+Proof.
+    induction s1; intros;
+        try rewrite app_length in *; simpl in *; split.
+    - apply Nat.le_0_l.
+    - assumption.
+    - rewrite length_app_distr, Nat.add_comm, plus_n_Sm in H. 
+		apply plus_le in H. now destruct H.
+	- rewrite length_app_distr, Nat.add_comm, plus_n_Sm in H.
+		apply plus_le in H. now destruct H.
+Qed.
+
+Lemma app_nil :
+    forall s1 s2,
+    "" = s1 ++ s2 -> s1 = "" /\ s2 = "".
+Proof.
+    induction s1; intros; simpl in *; split.
+    - reflexivity.
+    - symmetry. assumption.
+    - inversion H.
+    - inversion H.
+Qed.
+
+Lemma cons_inj : 
+    forall s1 s2 x,
+    s1 = s2 -> (String x s1) = (String x s2).
+Proof.
+    destruct s1; intros; now rewrite H. 
+Qed.
+
+Lemma app_single_end :
+    forall x s1 s2,
+    s1 ++ (String x "") = s2 ++ (String x "") -> s1 = s2.
+Proof.
+    induction s1; intros; simpl in *.
+    - destruct s2. reflexivity.
+        inversion H; subst.
+        destruct (app_nil s2 (String a "") H2); subst.
+        now symmetry.
+    - destruct s2; simpl in *.
+        inversion H; subst. 
+        symmetry in H2. 
+        destruct (app_nil s1 (String x "") H2); subst.
+        inversion H1. inversion H.
+        now apply cons_inj, IHs1.
+Qed.
+
+Lemma length_0_nil: forall s,
+    String.length s = 0%nat -> s = EmptyString.
+Proof.
+    destruct s. reflexivity. intro. inversion H.
+Qed.
+
+Lemma palindrome_step : 
+    forall n s,
+    (String.length s <= n)%nat -> s = reverse s -> pal s.
+Proof.
+    induction n; intros.
+    - inversion H. rewrite (length_0_nil s H2).
+        apply pal_nil.
+    - destruct s as [| hd tl]. 
+        -- apply pal_nil.
+        -- destruct (split_last tl); subst.
+            apply pal_single.
+            destruct H1 as [last], H1 as [mid]; subst.
+            simpl in *. apply le_S_n in H.
+			rewrite rev_String, reverse_app_distr in H0; simpl in *.
+            inversion H0. apply pal_ht.
+            apply IHn. apply length_app_le in H.
+            now destruct H.
+            now apply app_single_end in H3.
+Qed.
+
+Theorem palindrome_converse: forall s,
+    s = reverse s -> pal s.
+Proof.
+    intros. apply (palindrome_step (String.length s) s). 
+    subst. apply le_n.
+    assumption.
+Qed.
+
+Require Import Lia.
+Require Import BinPosDef.
+(* Open Scope positive_scope. *)
+
+(* Eval unfold ispalindrome in ispalindrome. *)
+
+Require Import FunctionalExtensionality.
+
+Lemma update_shadow : forall (m : store) x v1 v2,
+  (x !-> v2 ; x !-> v1 ; m) = (x !-> v2 ; m).
+Proof.
+  intros. apply functional_extensionality. intros.
+  unfold update. destruct (String.eqb x0 x) eqn:E; reflexivity.
+Qed.
+
+Lemma update_eq : forall (m : store) x v,
+	(x !-> v; m) x = v.
+Proof.
+	intros. unfold update. now rewrite String.eqb_refl.
+Qed.
+
+Lemma get_string_eq : forall m x v,
+	get_string (x !-> VString v; m) x = v. Admitted.
+
+Lemma get_int_eq : forall m x v,
+	get_int (x !-> VInteger v; m) x = v. Admitted.
+
+Lemma eqb_neq : forall (s1 s2 : string),
+	s1 <> s2 <-> (s1 =? s2)%string = false.
+Proof.
+	split; generalize dependent s2; induction s1; intros.
+	- destruct s2. now contradict H. reflexivity.
+	- destruct s2. reflexivity. destruct (Ascii.eqb a a0) eqn:E; simpl; rewrite E.
+		apply IHs1. intro. subst. assert (a <> a0). intro. subst. contradiction.
+		destruct (Ascii.eqb_neq a a0). rewrite (H2 H0) in E. inversion E. easy.
+	- destruct s2. inversion H. intro. inversion H0.
+	- intro. subst. simpl in H. rewrite Ascii.eqb_refl, String.eqb_refl in H. 
+		inversion H.
+Qed.
+
+Lemma update_neq : forall (m : store) x y v,
+	x <> y ->
+	(x !-> v; m) y = m y.
+Proof.
+	intros. unfold update. destruct (eqb_neq x y). now rewrite String.eqb_sym, (H0 H).
+Qed.
+
+(* Compute fst (ispalindrome (update fresh_store "VP_STR" (VString "")) 5000) "VP_result". *)
+
+Definition output_safe (f : store -> nat -> store * bool) 
+		input expected :=
+	forall loop_limit output, 
+		(output, false) = f input loop_limit -> output "VP_result" = expected.
+
+Theorem ispalindrome_small : forall s,
+	(String.length s <= 1)%nat ->
+	output_safe ispalindrome (update fresh_store "VP_STR" (VString s)) (VInteger 1).
+Proof.
+	intros s Small loop_limit output Terminates.
+	assert (s = "" \/ (exists x, s = (String x ""))) as Size.
+		destruct s. now left. right. exists a. destruct s. easy.
+		simpl in Small. lia.
+	destruct Size; [idtac|destruct H]; subst; destruct loop_limit; inversion Terminates;
+		now rewrite update_neq, update_neq, update_eq.
+Qed.
+
+Ltac vpex_term term := 
+	match term with [(?fst, ?snd) = 
+			match ?m with (Some s) => ?s' | None => ?n' end] => idtac s
+	end.
+
+Ltac vpex :=
+	match goal with [H: (?fst, ?snd) = 
+		match ?m with (Some s) => ?s' | None => ?n' end |- _] =>
+			let name := fresh "body" in
+			remember m as name
+	end || idtac "No match".
+
+Theorem ispalindrome_ht : forall h t,
+	pal t ->
+	output_safe ispalindrome 
+		(update fresh_store "VP_STR" (VString (String h t ++ (String h "")))) 
+		(VInteger 1).
+Proof.
+	intros h t Pal loop_limit.
+	revert Pal. induction loop_limit; intros Pal output Terminates.
+	- inversion Terminates.
+	- inversion Pal; subst. 
+		-- clear IHloop_limit. unfold ispalindrome in Terminates.
+			simpl in Terminates. vpex. rewrite get_int_eq in Heqbody.
+			repeat unfold get_string at 5 in Heqbody;
+				rewrite update_neq, update_neq, update_neq, update_eq in Heqbody; 
+					try discriminate.
+			repeat unfold string_subscript at 5 in Heqbody; simpl in Heqbody.
+			unfold Z_noteqb in Heqbody. rewrite Z.eqb_refl in Heqbody.
+				simpl in Heqbody. rewrite update_shadow in Heqbody.
+			destruct loop_limit. subst. inversion Terminates.
+			repeat rewrite get_int_eq in Heqbody.
+			unfold get_int at 1 in Heqbody. rewrite update_neq, 
+				update_eq in Heqbody; try discriminate.
+			simpl in Heqbody. subst. inversion Terminates.
+			rewrite update_neq, update_neq, update_eq; easy.
+		-- apply (IHloop_limit Pal). clear Terminates IHloop_limit.
+			induction (String x ""). (* last goal *) admit.
+
+			
+			
+
+(* Theorem ispalindrome (update fresh_store "VP_STR" (VString "")) "VP_result" = VInteger 1. *)
+
+Lemma neqb_refl : forall x,
+	x !=? x = false.
+Proof.
+	intros. unfold Z_noteqb. now rewrite Z.eqb_refl.
+Qed.
+
+Hint Unfold get_int.
+Hint Unfold get_string.
+
+Definition palindrome_partial_correctness : 
+	forall (s : string),
+	pal s -> output_safe ispalindrome (update fresh_store "VP_STR" (VString s)) (VInteger 1).
+Proof.
+	(* intros. intros loop_limit output Terminates. induction loop_limit.
+		inversion Terminates.
+		unfold ispalindrome in Terminates. simpl in Terminates.
+		unfold get_int in Terminates. rewrite 
+			update_eq, update_neq, update_eq in Terminates; try discriminate.
+		unfold get_string in Terminates at 1. rewrite 
+			update_neq, update_eq in Terminates; try discriminate.
+	destruct s. 
+	- inversion Terminates. now rewrite update_neq, update_neq, update_eq.
+	- destruct s. inversion Terminates. now rewrite update_neq, update_neq, update_eq.
+		assert (1 <=?
+		Z.of_nat
+		  (String.length (String a (String a0 s))) /
+		2 = true). clear H Terminates IHloop_limit. induction s. auto.
+		 *)
+	intros. intros loop_limit output Terminates. induction H; subst.
+	- apply ispalindrome_small in Terminates; auto.
+	- apply ispalindrome_small in Terminates; auto.
+	- induction loop_limit; inversion Terminates. unfold ispalindrome in Terminates.
+		simpl in *. unfold get_int in Terminates. 
+		rewrite update_eq, update_neq, update_eq in Terminates.
+		destruct (1 <=? _) in Terminates. vpex_term Terminates.
+		
+
+		inversion Terminates. rewrite update_neq, update_neq, update_eq.
+			auto. all: discriminate.
+
+	
