theories/Volpic_notation.v
@@ -3,9 +3,13 @@ Require Import Volpic_preamble.
 Declare Scope volpic_notation.
 Open Scope volpic_notation.
 
+Notation "'_' '!->' v" := (fresh_store v)
+    (at level 100, right associativity) : volpic_notation.
+Notation "x '!->' y ';' f" := (update f x y)
+    (at level 100, y at next level, right associativity) : volpic_notation.
+
 Notation "'while' '(' condition ')' 'with' store_name 'upto' loop_limit 'begin' loop_body 'end'" :=
-    (let body := loop_body in 
-        (fix loop (depth : nat) (broken : bool) (VP_store : store) :=
+    ((fix loop (depth : nat) (broken : bool) (VP_store : store) :=
         match depth with 
         | O => None
         | S n' => 
